new/proof/std.v
@@ -39,13 +39,13 @@ Context `{!std.GlobalAddrs}.
   automatically included here).
  *)
 #[global]
-Program Instance : IsPkgInit std.pkg_name' :=
+Program Instance : IsPkgInit std :=
   ltac2:(build_pkg_init ()).
 Final Obligation. apply _. Qed.
 
 Lemma wp_Assert (cond : bool) :
-  {{{ is_pkg_init std.pkg_name' ∗ ⌜cond = true⌝ }}}
-    func_call #std.pkg_name' #"Assert" #cond
+  {{{ is_pkg_init std ∗ ⌜cond = true⌝ }}}
+    func_call #std #"Assert" #cond
   {{{ RET #(); True }}}.
 Proof.
   wp_start as "%". subst.
@@ -54,8 +54,8 @@ Proof.
 Qed.
 
 Lemma wp_SumNoOverflow (x y : u64) :
-  {{{ is_pkg_init std.pkg_name' }}}
-    func_call #std.pkg_name' #"SumNoOverflow" #x #y
+  {{{ is_pkg_init std }}}
+    func_call #std #"SumNoOverflow" #x #y
   {{{ RET #(bool_decide (uint.Z (word.add x y) = (uint.Z x + uint.Z y)%Z)); True }}}.
 Proof.
   wp_start as "_".
@@ -69,8 +69,8 @@ Proof.
 Qed.
 
 Lemma wp_SumAssumeNoOverflow (x y : u64) :
-  {{{ is_pkg_init std.pkg_name' }}}
-    func_call #std.pkg_name' #"SumAssumeNoOverflow" #x #y
+  {{{ is_pkg_init std }}}
+    func_call #std #"SumAssumeNoOverflow" #x #y
   {{{ RET #(word.add x y); ⌜uint.Z (word.add x y) = (uint.Z x + uint.Z y)%Z⌝ }}}.
 Proof.
   wp_start as "_".
@@ -86,7 +86,7 @@ Definition is_JoinHandle (l: loc) (P: iProp Σ): iProp _ :=
   ∃ (mu_l cond_l: loc),
   "#mu" ∷ l ↦s[std.JoinHandle :: "mu"]□ mu_l ∗
   "#cond" ∷ l ↦s[std.JoinHandle :: "cond"]□ cond_l ∗
-  "#Hcond" ∷ is_Cond cond_l (interface.mk sync.pkg_name' "Mutex'ptr"%go #mu_l) ∗
+  "#Hcond" ∷ is_Cond cond_l (interface.mk sync "Mutex'ptr"%go #mu_l) ∗
   "#Hlock" ∷ is_Mutex mu_l
      (∃ (done_b: bool),
          "done_b" ∷ l ↦s[std.JoinHandle :: "done"] done_b ∗
@@ -94,8 +94,8 @@ Definition is_JoinHandle (l: loc) (P: iProp Σ): iProp _ :=
 .
 
 Lemma wp_newJoinHandle (P: iProp Σ) :
-  {{{ is_pkg_init std.pkg_name' }}}
-    func_call #std.pkg_name' #"newJoinHandle" #()
+  {{{ is_pkg_init std }}}
+    func_call #std #"newJoinHandle" #()
   {{{ (l: loc), RET #l; is_JoinHandle l P }}}.
 Proof.
   wp_start as "_".
@@ -124,8 +124,8 @@ Proof.
 Qed.
 
 Lemma wp_JoinHandle__finish l (P: iProp Σ) :
-  {{{ is_pkg_init std.pkg_name' ∗ is_JoinHandle l P ∗ P }}}
-    method_call #std.pkg_name' #"JoinHandle'ptr" #"finish" #l #()
+  {{{ is_pkg_init std ∗ is_JoinHandle l P ∗ P }}}
+    method_call #std #"JoinHandle'ptr" #"finish" #l #()
   {{{ RET #(); True }}}.
 Proof.
   wp_start as "[Hhandle P]".
@@ -144,9 +144,9 @@ Proof.
 Qed.
 
 Lemma wp_Spawn (P: iProp Σ) (f : func.t) :
-  {{{ is_pkg_init std.pkg_name' ∗
+  {{{ is_pkg_init std ∗
         (∀ Φ, ▷(P -∗ Φ #()) -∗ WP #f #() {{ Φ }}) }}}
-  func_call #std.pkg_name' #"Spawn" #f
+  func_call #std #"Spawn" #f
   {{{ (l: loc), RET #l; is_JoinHandle l P }}}.
 Proof.
   wp_start as "Hwp".
@@ -173,8 +173,8 @@ Proof.
 Qed.
 
 Lemma wp_JoinHandle__Join l P :
-  {{{ is_pkg_init std.pkg_name' ∗ is_JoinHandle l P }}}
-    method_call #std.pkg_name' #"JoinHandle'ptr" #"Join" #l #()
+  {{{ is_pkg_init std ∗ is_JoinHandle l P }}}
+    method_call #std #"JoinHandle'ptr" #"Join" #l #()
   {{{ RET #(); P }}}.
 Proof.
   wp_start as "Hjh". iNamed "Hjh".
