new/proof/context.v
@@ -37,7 +37,7 @@ Context `{hG: heapGS Σ, !ffi_semantics _ _}.
 Context `{!goGlobalsGS Σ}.
 
 #[global]
-Program Instance : IsPkgInit context.pkg_name' :=
+Program Instance : IsPkgInit context :=
   ltac2:(build_pkg_init ()).
 Final Obligation. Proof. apply _. Qed.
 
@@ -73,7 +73,7 @@ then (cancel was run) ∨ (chan.is_closed ctx.Done). *)
 
 Lemma wp_WithCancel N (ctx : interface.t) :
   {{{ True }}}
-    func_call #context.pkg_name' #"WithCancel" #ctx
+    func_call #context #"WithCancel" #ctx
   {{{
         ctx' ctx_state (cancel : func.t), RET (#ctx', #cancel);
         is_Context ctx' ctx_state ∗
