new/proof/sync/atomic.v
@@ -9,15 +9,15 @@ Context `{!goGlobalsGS Σ}.
 Context `{!atomic.GlobalAddrs}.
 
 #[global]
-Program Instance is_pkg_init_inst : IsPkgInit atomic.pkg_name' :=
+Program Instance is_pkg_init_inst : IsPkgInit atomic :=
   ltac2:(build_pkg_init ()).
 Final Obligation. apply _. Qed.
 
 Lemma wp_LoadUint64 (addr : loc) dq :
   ∀ Φ,
-  is_pkg_init atomic.pkg_name' -∗
+  is_pkg_init atomic -∗
   (|={⊤,∅}=> ∃ (v : w64), addr ↦{dq} v ∗ (addr ↦{dq} v ={∅,⊤}=∗ Φ #v)) -∗
-  WP func_call #atomic.pkg_name' #"LoadUint64" #addr {{ Φ }}.
+  WP func_call #atomic #"LoadUint64" #addr {{ Φ }}.
 Proof.
   wp_start as "_".
   iMod "HΦ" as (?) "[Haddr HΦ]".
@@ -26,9 +26,9 @@ Qed.
 
 Lemma wp_StoreUint64 (addr : loc) (v : w64) :
   ∀ Φ,
-  is_pkg_init atomic.pkg_name' -∗
+  is_pkg_init atomic -∗
   (|={⊤,∅}=> ∃ (oldv : w64), addr ↦ oldv ∗ (addr ↦ v ={∅,⊤}=∗ Φ #())) -∗
-  WP func_call #atomic.pkg_name' #"StoreUint64" #addr #v {{ Φ }}.
+  WP func_call #atomic #"StoreUint64" #addr #v {{ Φ }}.
 Proof.
   wp_start as "_".
   iMod "HΦ" as (?) "[Haddr HΦ]".
@@ -37,22 +37,22 @@ Qed.
 
 Lemma wp_AddUint64 (addr : loc) (v : w64) :
   ∀ Φ,
-  is_pkg_init atomic.pkg_name' -∗
+  is_pkg_init atomic -∗
   (|={⊤,∅}=> ∃ (oldv : w64), addr ↦ oldv ∗ (addr ↦ (word.add oldv v) ={∅,⊤}=∗ Φ #(word.add oldv v))) -∗
-  WP func_call #atomic.pkg_name' #"AddUint64" #addr #v {{ Φ }}.
+  WP func_call #atomic #"AddUint64" #addr #v {{ Φ }}.
 Proof.
 Admitted.
 
 Lemma wp_CompareAndSwapUint64 (addr : loc) (old : w64) (new : w64) :
   ∀ Φ,
-  is_pkg_init atomic.pkg_name' -∗
+  is_pkg_init atomic -∗
   (|={⊤,∅}=>
      ∃ (v: w64) dq,
      addr ↦{dq} v ∗
      ⌜ dq = if decide (v = old) then DfracOwn 1 else dq ⌝ ∗
      (addr ↦{dq} (if decide (v = old) then new else v) ={∅,⊤}=∗ Φ #(bool_decide (v = old)))
   ) -∗
-  WP func_call #atomic.pkg_name' #"CompareAndSwapUint64" #addr #old #new {{ Φ }}.
+  WP func_call #atomic #"CompareAndSwapUint64" #addr #old #new {{ Φ }}.
 Proof.
   wp_start as "_".
   wp_bind (CmpXchg _ _ _).
@@ -78,9 +78,9 @@ Definition own_Uint64 (u : loc) dq (v : w64) : iProp Σ :=
 
 Lemma wp_Uint64__Load u dq :
   ∀ Φ,
-  is_pkg_init atomic.pkg_name' -∗
+  is_pkg_init atomic -∗
   (|={⊤,∅}=> ∃ v, own_Uint64 u dq v ∗ (own_Uint64 u dq v ={∅,⊤}=∗ Φ #v)) -∗
-  WP method_call #atomic.pkg_name' #"Uint64'ptr" #"Load" #u #() {{ Φ }}.
+  WP method_call #atomic #"Uint64'ptr" #"Load" #u #() {{ Φ }}.
 Proof.
   wp_start as "_".
   wp_alloc x_ptr as "Hx_ptr".
@@ -106,9 +106,9 @@ Qed.
 
 Lemma wp_Uint64__Store u v :
   ∀ Φ,
-  is_pkg_init atomic.pkg_name' -∗
+  is_pkg_init atomic -∗
   (|={⊤,∅}=> ∃ old, own_Uint64 u (DfracOwn 1) old ∗ (own_Uint64 u (DfracOwn 1) v ={∅,⊤}=∗ Φ #())) -∗
-  WP method_call #atomic.pkg_name' #"Uint64'ptr" #"Store" #u #v {{ Φ }}.
+  WP method_call #atomic #"Uint64'ptr" #"Store" #u #v {{ Φ }}.
 Proof.
   wp_start as "_".
   wp_alloc x_ptr as "Hx_ptr". wp_pures.
@@ -136,11 +136,11 @@ Qed.
 
 Lemma wp_Uint64__Add u delta :
   ∀ Φ,
-  is_pkg_init atomic.pkg_name' -∗
+  is_pkg_init atomic -∗
   (|={⊤,∅}=> ∃ old, own_Uint64 u (DfracOwn 1) old ∗
   (own_Uint64 u (DfracOwn 1) (word.add old delta) ={∅,⊤}=∗
    Φ #(word.add old delta))) -∗
-  WP method_call #atomic.pkg_name' #"Uint64'ptr" #"Add" #u #delta {{ Φ }}.
+  WP method_call #atomic #"Uint64'ptr" #"Add" #u #delta {{ Φ }}.
 Proof.
   wp_start as "_".
   wp_alloc new_ptr as "Hnew_ptr". wp_pures.
@@ -168,11 +168,11 @@ Qed.
 
 Lemma wp_Uint64__CompareAndSwap u old new :
   ∀ Φ,
-  is_pkg_init atomic.pkg_name' -∗
+  is_pkg_init atomic -∗
   (|={⊤,∅}=> ∃ v dq, own_Uint64 u dq v ∗
                     ⌜ dq = if decide (v = old) then DfracOwn 1 else dq ⌝ ∗
   (own_Uint64 u dq (if decide (v = old) then new else v) ={∅,⊤}=∗ Φ #(bool_decide (v = old)))) -∗
-  WP method_call #atomic.pkg_name' #"Uint64'ptr" #"CompareAndSwap" #u #old #new {{ Φ }}.
+  WP method_call #atomic #"Uint64'ptr" #"CompareAndSwap" #u #old #new {{ Φ }}.
 Proof.
   wp_start as "_".
   wp_alloc swapped_ptr as "Hswapped_ptr". wp_pures.
